theories/LambdaWPTactics.v
@@ -780,4 +780,4 @@ then just:
 *)
 
 
-End Test.
+End Test.Z.a
